<?xml version="1.0"?>


<!DOCTYPE rdf:RDF [
    <!ENTITY owl "http://www.w3.org/2002/07/owl#" >
    <!ENTITY xsd "http://www.w3.org/2001/XMLSchema#" >
    <!ENTITY owl2xml "http://www.w3.org/2006/12/owl2-xml#" >
    <!ENTITY rdfs "http://www.w3.org/2000/01/rdf-schema#" >
    <!ENTITY rdf "http://www.w3.org/1999/02/22-rdf-syntax-ns#" >
    <!ENTITY Ontology1265975763515 "http://www.semanticweb.org/ontologies/2010/1/Ontology1265975763515.owl#" >
]>


<rdf:RDF xmlns="http://www.semanticweb.org/ontologies/2010/1/Ontology1265975763515.owl#"
     xml:base="http://www.semanticweb.org/ontologies/2010/1/Ontology1265975763515.owl"
     xmlns:rdfs="http://www.w3.org/2000/01/rdf-schema#"
     xmlns:owl2xml="http://www.w3.org/2006/12/owl2-xml#"
     xmlns:owl="http://www.w3.org/2002/07/owl#"
     xmlns:xsd="http://www.w3.org/2001/XMLSchema#"
     xmlns:rdf="http://www.w3.org/1999/02/22-rdf-syntax-ns#"
     xmlns:Ontology1265975763515="http://www.semanticweb.org/ontologies/2010/1/Ontology1265975763515.owl#">
    <owl:Ontology rdf:about=""/>
    


    <!-- 
    ///////////////////////////////////////////////////////////////////////////////////////
    //
    // Classes
    //
    ///////////////////////////////////////////////////////////////////////////////////////
     -->


    <owl:Class rdf:about="#WikiDiscussionItem">
    	<rdfs:label>Wiki Discussion Item</rdfs:label> 
        <rdfs:comment>A single contribution to the discussion on a wiki Talk page.</rdfs:comment>	
    </owl:Class>
    
    
    <owl:Class rdf:about="ReferenceItem">
    	<rdfs:label>Reference Item</rdfs:label> 
    	<rdfs:subClassOf>WikiDiscussionItem</rdfs:subClassOf>
    	<rdfs:comment>A WikiDiscussionItem that refers to something else.</rdfs:comment>	
    </owl:Class>
    

    <owl:Class rdf:about="RequestItem">
        <rdfs:label>Request Item</rdfs:label>
    	<rdfs:subClassOf>WikiDiscussionItem</rdfs:subClassOf>
    	<rdfs:comment>A WikiDiscussionItem that requests something.</rdfs:comment>	
    </owl:Class>
    

    <owl:Class rdf:about="#RequestEditingCoordination">
        <rdfs:subClassOf>RequestItem</rdfs:subClassOf>
        <rdfs:label>Requests/suggestions for editing coordination</rdfs:label>
        <rdfs:comment>Ideas, comments, or suggestions involving editing the article.</rdfs:comment>	
    </owl:Class>
    
    
    <owl:Class rdf:about="#ReferenceToGuidelinesOrPolicies">
        <rdfs:subClassOf>ReferenceItem</rdfs:subClassOf>
        <rdfs:label>References to guidelines and policies of this wiki.</rdfs:label>
        <rdfs:comment></rdfs:comment>	
    </owl:Class>
    
    
    <owl:Class rdf:about="#RequestInfo">
        <rdfs:subClassOf>RequestItem</rdfs:subClassOf>
        <rdfs:label>Requests for information</rdfs:label>
        <rdfs:comment>Questions asked by someone who does not intend to edit the page.</rdfs:comment>	
    </owl:Class>
    
    
    <owl:Class rdf:about="#ReferenceToInternalResources">
        <rdfs:subClassOf>ReferenceItem</rdfs:subClassOf>                
        <rdfs:label>References to internal resources of this wiki</rdfs:label>
        <rdfs:comment>References to internal wiki resources such as diffs, Talk page discussions, old version of a page, etc.</rdfs:comment>	
    </owl:Class>
    

    <owl:Class rdf:about="#ReferenceToEdit">
        <rdfs:subClassOf>ReferenceItem</rdfs:subClassOf>
        <rdfs:label>Reference to edits the discussant made</rdfs:label>
        <rdfs:comment>Applied when an editor discusses his/her own article edits on the Talk page.</rdfs:comment>	
    </owl:Class>
    
    
    <owl:Class rdf:about="#RequestPeer-review">
        <rdfs:subClassOf>RequestItem</rdfs:subClassOf>
        <rdfs:label>Requests for peer review</rdfs:label>
        <rdfs:comment>Viegas 2007 explains this category: "Users hoping to elevate articles to featured status may solicit a peer review."</rdfs:comment>	
    </owl:Class>


	<owl:Class rdf:about="#RequestHelpElsewhere">
        <rdfs:subClassOf>RequestItem</rdfs:subClassOf>
        <rdfs:label>Requests for help with another article, portal, etc.</rdfs:label>
        <rdfs:comment>Recruiting editorial help in this Talk page for other pages (not this article), such as the article on another subject, a portal, WikiProject, etc.</rdfs:comment>	
    </owl:Class>
    

    <owl:Class rdf:about="#ReferenceToRevertsOrControversialOrRemovedMaterial">
        <rdfs:subClassOf>ReferenceItem</rdfs:subClassOf>
        <rdfs:label>References to reverts, removed material, or controversial edits</rdfs:label>
        <rdfs:comment>Discussions of reverts, removing material, or controversial edits.</rdfs:comment>	
    </owl:Class>
    
    
    <owl:Reference rdf:about="#ReferenceToSources">
        <rdfs:subClassOf>ReferenceItem</rdfs:subClassOf>
        <rdfs:label>References to sources outside Wiki</rdfs:label>
        <rdfs:comment>References to sources, including print and deep web resources, outside this wiki.</rdfs:comment>	
    </owl:Reference>
    

    <owl:Class rdf:about="#ReferenceToVandalism">
        <rdfs:subClassOf>ReferenceItem</rdfs:subClassOf>
        <rdfs:label>References to vandalism</rdfs:label>
        <rdfs:comment>Mentions of vandalism or purported vandalism.</rdfs:comment>	
    </owl:Class>
    
</rdf:RDF>
